Added comments on completeness, started to look at correctness

CEval.v
@@ -62,33 +62,33 @@ Module CEvalStep.
    
    Open Scope stm_scope. (*to avoid writing %stm after each statement*)
   
-   Reserved Notation " t '/' st '-->' t' '/' st' " (at level 40, st at level 39, t' at level 39).
+   Reserved Notation "'(||' st ',' t '||)' '-->c' '(||' st' ',' t' '||)'" (at level 40, st at level 39, t' at level 39).
    (*CEval -> we have a small step evaluation here represented by a relation*)
-    Inductive cstep : (statement * state) -> (statement * state) -> Prop :=
+    Inductive cstep : (state * statement) -> (state * statement) -> Prop :=
     | CS_Ass : forall st i a,
-        (i ::= a) / st --> (SKIP) / (i !-> (aeval st a) ; st) 
+        (|| st, i ::= a ||) -->c (|| (i !-> (aeval st a) ; st), SKIP ||)
     | CS_SeqStep : forall st s1 s1' s2 st',
-        s1 / st --> s1' / st' ->
-        (s1 ;; s2) / st --> (s1' ;; s2) / st'
+        (|| st, s1 ||) -->c (|| st', s1' ||) ->
+        (|| st, s1 ;; s2 ||)-->c (|| st', s1' ;; s2 ||)
     | CS_SeqFinish : forall st s2,
-        (SKIP ;; s2) / st --> s2 / st 
+        (|| st, SKIP ;; s2 ||) -->c (|| st, s2 ||) 
     | CS_IfTrue : forall st s1 s2 b,
         (beval st b) = true ->
-        (If b THEN s1 ELSE s2) / st --> s1 / st
+        (|| st, If b THEN s1 ELSE s2 ||) -->c (|| st, s1 ||)
     | CS_IfFalse : forall st s1 s2 b,
         (beval st b) = false ->
-        (If b THEN s1 ELSE s2) / st --> s2 / st
+        (|| st, If b THEN s1 ELSE s2 ||) -->c (|| st, s2 ||)
     | CS_While : forall st b s,
-        (WHILE b DO s END) / st -->
-                           (If b THEN (s ;; (WHILE b DO s END)) ELSE SKIP) / st
+        (|| st, WHILE b DO s END ||) -->c
+        (|| st, If b THEN (s ;; (WHILE b DO s END)) ELSE SKIP ||)
     | CS_N0While : forall st b n s,
         n = 0 ->
-        (WHILE b FOR n DO s END) / st -->
-                           (SKIP) / st
+        (|| st, WHILE b FOR n DO s END ||) -->c
+        (|| st,  SKIP ||)
      | CS_NWhile : forall st b n s,
-        (WHILE b FOR n DO s END) / st -->
-                           (If b THEN (s ;; (WHILE b FOR n-1 DO s END)) ELSE SKIP) / st
-    where " t '/' st '-->' t' '/' st' " := (cstep (t,st) (t',st')).  
+        (|| st, WHILE b FOR n DO s END ||) -->c
+        (|| st, If b THEN (s ;; (WHILE b FOR n-1 DO s END)) ELSE SKIP ||)
+    where "'(||' st ',' t '||)' '-->c' '(||' st' ',' t' '||)'" := (cstep (st,t) (st',t')).  
 
 (*The hints are simplifying the proofs for wach statement*)
 Hint Constructors cstep.
@@ -104,33 +104,33 @@ Inductive multi {X : Type} (R : relation X) : relation X :=
                     multi R x z.
 Hint Constructors multi.
 
-Notation " t '/' st '-->*' t' '/' st' " :=
-   (multi cstep  (t,st) (t',st'))
+Notation "'(||' st ',' t '||)' '-->c*' '(||' st' ',' t' '||)'" :=
+   (multi cstep  (st,t) (st',t'))
      (at level 40, st at level 39, t' at level 39).
 
 (*Examples illustrating how evaluation works*)
 Example cstep_ex_skip :
   forall st,
-    (SKIP) / st -->* (SKIP) / st .
+    (|| st, SKIP ||) -->c*  (|| st, SKIP ||) .
 Proof.
   auto. Qed. (*with Hint Constructors*) 
   (*intros st.
     apply multi_refl. Qed. -without hint constructors *)
 
 Example cstep_ex_asgn :
-    (Y ::= 3) / (X !-> 1) -->* (SKIP) / ( Y !-> 3 ; X !-> 1).
+    (|| (X !-> 1), Y ::= 3 ||)  -->c* (|| ( Y !-> 3 ; X !-> 1), SKIP ||).
 Proof.
   eauto. Qed. (*with hint constructors*) 
   (*eapply multi_step. {apply CS_Ass. }
                      apply multi_refl. Qed. (*without hint Constructors*) *)
 
 Example cstep_ex2_asgn :
-    (Y ::= 3) / (X !-> 1) --> (SKIP) / ( Y !-> 3 ; X !-> 1).
+    (|| (X !-> 1), Y ::= 3 ||)  -->c (|| ( Y !-> 3 ; X !-> 1), SKIP ||).
 Proof.
   apply CS_Ass. Qed.
 
 Example cstep_ex3_seq:
-  (X ::= 1  ;; Y ::= 3) / empty_st -->* (SKIP) / ( Y !-> 3; X !-> 1) .
+  (|| empty_st, (X ::= 1  ;; Y ::= 3) ||) -->c* (|| ( Y !-> 3; X !-> 1), SKIP ||) .
 
 Proof.
   eauto. Qed. (*with hint constructors*)
@@ -142,7 +142,7 @@ Proof.
   apply multi_refl. Qed. *) (*without*)
 
 Example cstep_ex4_if:
-  stm_if / empty_st -->* (SKIP) / ( Z !-> 5 ;  X !-> 1 ).
+  (|| empty_st, stm_if ||)-->c* (|| (Z !-> 5 ;  X !-> 1 ), SKIP ||).
 Proof.
   unfold stm_if.
   eapply multi_step. eapply CS_SeqStep. apply CS_Ass. simpl.
@@ -151,7 +151,7 @@ Proof.
   apply multi_refl. Qed.
 
 Example cstep_ex5_while:
-  stm_while / empty_st -->* (SKIP) / (X !-> 1 ; X !-> 0).
+  (|| empty_st, stm_while ||) -->c* (|| (X !-> 1 ; X !-> 0), SKIP ||).
 Proof.
   unfold stm_while.
   eapply multi_step. eapply CS_SeqStep. apply CS_Ass.
@@ -165,7 +165,7 @@ Proof.
   apply multi_refl. Qed.
 
 Example cstep_ex6_n_while:
-  stm_n_while / (X !-> 0) -->* (SKIP) / (X !-> 2 ; X !-> 1 ; X !-> 0).
+  (|| (X !-> 0), stm_n_while ||) -->c* (|| (X !-> 2 ; X !-> 1 ; X !-> 0), SKIP ||).
 Proof.
   unfold stm_n_while.
   eapply multi_step. eapply CS_NWhile.
@@ -179,32 +179,34 @@ Proof.
   eapply multi_refl. Qed.
  
     
-    Reserved Notation " t '/' st '-->t' t' '/' st' "
+    Reserved Notation "'(|' st ',' t '|)' '-->tc' '(|' st' ',' t' '|)'"
              (at level 40, st at level 39, t' at level 39).
 
     (*Non-deterministic evaluation when threads are involved*)
     (*Also a small step evaluation as a relation*)
-    Inductive tpstep : (threadPool * state) -> (threadPool * state) -> Prop :=
+    Inductive tpstep : (state * threadPool) -> (state * threadPool) -> Prop :=
     | TS_T1 : forall st t1 t1' t2 st',
-        t1 / st -->t t1' / st' ->
-        (TPar t1 t2) / st -->t (TPar t1' t2) / st'
+        (| st , t1 |) -->tc (| st' , t1' |) ->
+        (| st, TPar t1 t2 |) -->tc (| st', TPar t1' t2 |)
     | TS_T2 : forall st t1 t2 t2' st',
-        t2 / st -->t t2' / st' ->
-        (TPar t1  t2) / st -->t (TPar t1 t2') / st'
+        (| st, t2 |) -->tc (| st', t2' |) ->
+        (| st, TPar t1  t2 |) -->tc (| st', TPar t1 t2' |)
     | TS_ST1 : forall st s1 s1' st' n t2, (*when we arrive to statements*)
-        s1 / st --> s1' / st' ->
-        (TPar << id n | s1 >> t2) / st -->t (TPar << id n | s1' >> t2) / st'        
+        (|| st, s1 ||) -->c (|| st', s1' ||)  ->
+        (| st, TPar << id n | s1 >> t2 |) -->tc
+        (| st', TPar << id n | s1' >> t2 |)        
     | TS_ST2 : forall st s2 s2' st' t1 n, 
-        s2 / st --> s2' / st' ->
-        (TPar t1 << id n | s2 >>) / st -->t (TPar t1 << id n | s2' >>) / st'
+        (|| st, s2 ||) -->c (|| st', s2' ||) ->
+        (| st, TPar t1 << id n | s2 >> |) -->tc
+        (| st', TPar t1 << id n | s2' >> |)
     | TS_STDone : forall st n n',
-        (TPar << id n | SKIP >> << id n' | SKIP >>) / st -->t
-                                                    << id n | SKIP >> / st 
+        (| st, TPar << id n | SKIP >> << id n' | SKIP >> |) -->tc
+        (| st, << id n | SKIP >> |) 
         
-          where " t '/' st '-->t' t' '/' st' " := (tpstep (t, st) (t', st')).
+          where "'(|' st ',' t '|)' '-->tc' '(|' st' ',' t' '|)'" := (tpstep (st, t) (st', t')).
 
-Notation " t '/' st '-->t*' t' '/' st' " :=
-   (multi tpstep  (t,st) (t',st'))
+Notation "'(|' st ',' t '|)' '-->tc*' '(|' st' ',' t' '|)'" :=
+   (multi tpstep  (st,t) (st',t'))
      (at level 40, st at level 39, t' at level 39).
 
 (*Used in proof*)
@@ -215,7 +217,7 @@ Print ex_intro.
 the value of X is dependent on the execution order*)
 Example tpstep_ex1:
   exists st',
-       stm_thread / empty_st  -->t* << id 0 | SKIP >> / st'
+       (| empty_st, stm_thread |)  -->tc* (| st', << id 0 | SKIP >> |)
        /\ st' X = 0.
 Proof.
   eapply ex_intro. split.
@@ -240,14 +242,14 @@ Proof.
 
 Example tpstep_ex2:
   exists st',
-    stm_thread / empty_st -->t* Thread (id 0) (SKIP) /  st'
+    (| empty_st, stm_thread |) -->tc* (| st', << id 0 | SKIP >> |)
     /\ st' X = 1.
 Proof.
   eapply ex_intro. split. unfold stm_thread. 
   (*thread 2 first*)
   eapply multi_step. apply TS_ST2. apply CS_Ass.
 
-  (*then tread 1*)  
+  (*then tread 1*)
   eapply multi_step. apply TS_T1.
   (*thread 2 in thread 1 first*)
   apply TS_ST2. apply CS_While. 
@@ -266,8 +268,26 @@ Proof.
   apply multi_refl.
   reflexivity. Qed.
 
-Example tpstep_article:
-  example_article / ( X !-> 5; Y !-> 5 ) -->t* Thread (id 1) (SKIP) /  (X !->1 ; Y !-> 0 ; X !-> 0 ; X !-> 5; Y !-> 5).
+Example tpstep_article_ex1:
+  exists st st',
+    (| st, example_article |) -->tc* (| st', << id 1 | SKIP >>|).
+Proof.
+  unfold example_article.
+  exists empty_st, (X !->1 ; Y !-> 0; X !-> 0).  (*we give an example of concrete states*)
+  eapply multi_step. apply TS_ST1. apply CS_SeqStep. apply CS_Ass. simpl. 
+  eapply multi_step. apply TS_ST1. apply CS_SeqFinish.
+
+  eapply multi_step. apply TS_ST2. apply CS_IfTrue. simpl. reflexivity.
+  eapply multi_step. apply TS_ST2. apply CS_Ass. simpl.
+
+  eapply multi_step. apply TS_ST1. apply CS_Ass. simpl.
+
+  eapply multi_step. apply TS_STDone. apply multi_refl. Qed. 
+  
+
+(*Example tpstep_article:
+  (|| ( X !-> 5; Y !-> 5 ), example_article ||) -->tc*
+  (|| (X !->1 ; Y !-> 0 ; X !-> 0 ; X !-> 5; Y !-> 5), Thread (id 1) (SKIP) ||).
 Proof.
   unfold example_article.
   eapply multi_step. apply TS_ST1. apply CS_SeqStep. apply CS_Ass. simpl. 
@@ -278,7 +298,7 @@ Proof.
 
   eapply multi_step. apply TS_ST1. apply CS_Ass. simpl.
 
-  eapply multi_step. apply TS_STDone. apply multi_refl. Qed. 
+  eapply multi_step. apply TS_STDone. apply multi_refl. Qed. *)
 
   
 Close Scope stm_scope.
