SymEval.v
@@ -21,14 +21,19 @@ symExprArit as type*)
 Open Scope symexpr. 
 Definition sym_state := total_map symExprArit.
 (*default value*)
-Definition empty_sym_st := (_ !-> SymNat(0)).
-Check empty_sym_st.
+Notation "'_' '|->' v" := (t_empty v) (at level 100, right associativity).
+Notation "x '|->' v ';' m" := (t_update m x v)
+                              (at level 100, v at next level, right associativity).
+
+Definition empty_sym_st := (_ |-> SymNat(0)).
+Check empty_sym_st. 
 
 (*Classic notation for maps*)
-Notation "a '!->' x" := (t_update empty_sym_st a x) (at level 100).
+Notation "a '|->' x" := (t_update empty_sym_st a x) (at level 100).
 Compute empty_sym_st .
 Compute empty_sym_st "x"%string .
-Compute (X !-> x(0) + 3 ; X !-> x(0); empty_sym_st) X .
+Compute (X |-> x(0) + 3 ; X |-> x(0); empty_sym_st) X .
+Check ( X !-> 0). (*string -> nat, but it goes through the notation defined here...*)
   
 (*symbolic evaluation of arithmetic expressions*)
 Fixpoint sym_aeval(st : sym_state) (t : aexpr) : symExprArit :=
@@ -41,9 +46,10 @@ Fixpoint sym_aeval(st : sym_state) (t : aexpr) : symExprArit :=
   end.
 
 
-Compute sym_aeval (X !-> x(0) ; Y !-> y(0)) ((X + 1 + Y) * X ).
+Compute sym_aeval (X |-> x(0) ; Y |-> y(0)) ((X + 1 + Y) * X ).
+
 (*adding constant folding would be nice*)
-Compute sym_aeval (X !-> (x(0) + 2 + 3)) X.
+Compute sym_aeval (X |-> (x(0) + 2 + 3)) X.
 
 (*symbolic evaluation of boolean expressions*)
 Fixpoint sym_beval(st : sym_state) (t : bexpr) : symExprBool :=
@@ -77,7 +83,7 @@ Fixpoint vars_bool (t : bexpr) : list string :=
   end.
 
 Compute vars_bool ( ((X + 1 + Y) * X) = 2).
-Compute (sym_beval (X !-> x(5)) (3 = X + 5)).
+Compute (sym_beval (X |-> x(5)) (3 = X + 5)).
 
 (*I need to get the conditions!*)
 Check [1].
@@ -101,65 +107,65 @@ Open Scope stm_scope.
 
 (*Issue: how to go from SymExprBool to bool - What is true???*)
 
-Reserved Notation "'(||' t ',' sp ',' st '||)' '--[' l ']-->s' '(||' t' ',' sp' ',' st' '||)'"
+Reserved Notation "'(||' st ',' sp ',' t '||)' '--[' l ']-->s' '(||' st' ',' sp' ',' t' '||)'"
          (at level 40, st at level 39, t' at level 39). 
 
-Inductive sym_step : tid -> (statement  * symPath * sym_state) ->
-                            (statement * symPath * sym_state) -> Prop :=
+Inductive sym_step : tid -> (sym_state  * symPath * statement) ->
+                            (sym_state * symPath * statement) -> Prop :=
     | S_Ass : forall st i a l sp,
-        (|| i::= a, sp, st ||) --[l]-->s
-        (|| SKIP, sp ++ [l⟨SymBool true, [i], vars_arit a⟩], (i !-> sym_aeval st a ; st) ||)
+        (|| st, sp, i ::= a ||) --[l]-->s
+        (|| (i |-> sym_aeval st a ; st), sp ++ [l⟨SymBool true, [i], vars_arit a⟩], SKIP ||)
 
     | S_SeqStep : forall st s1 s1' s2 l sp sp' st',
-        (|| s1, sp, st ||) --[l]-->s (|| s1', sp', st' ||) ->
-        (|| s1 ;; s2, sp, st ||) --[l]-->s
-        (|| s1' ;; s2 , sp', st' ||)
+        (|| st, sp, s1 ||) --[l]-->s (|| st', sp', s1' ||) ->
+        (|| st, sp, s1 ;; s2 ||) --[l]-->s
+        (|| st', sp', s1' ;; s2 ||)
 
     | S_SeqFinish : forall st s2 l sp,
-        (|| SKIP ;; s2, sp, st ||) --[l]-->s
-        (|| s2, sp, st ||)
+        (|| st, sp, SKIP ;; s2 ||) --[l]-->s
+        (|| st, sp, s2 ||)
 
     | S_IfTrue : forall st b s1 s2 l sp,
-        (|| If b THEN s1 ELSE s2, sp, st ||) --[l]-->s
-        (|| s1, sp ++ [l⟨sym_beval st b, [], vars_bool b⟩], st ||)
+        (|| st, sp, If b THEN s1 ELSE s2 ||) --[l]-->s
+        (|| st, sp ++ [l⟨sym_beval st b, [], vars_bool b⟩], s1 ||)
         
     | S_IfFalse : forall st b s1 s2 l sp,
-        (|| If b THEN s1 ELSE s2, sp, st ||) --[l]-->s
-        (|| s2, sp ++  [l⟨SymNot (sym_beval st b), [], vars_bool b⟩], st ||)
+        (|| st, sp, If b THEN s1 ELSE s2 ||) --[l]-->s
+        (|| st, sp ++  [l⟨SymNot (sym_beval st b), [], vars_bool b⟩], s2 ||)
 
-    | S_WhileTrue : forall st b s l sp,
-        (|| WHILE b DO s END, sp, st ||) --[l]-->s
-        (|| WHILE b DO s END, sp ++ [l⟨sym_beval st b, [], vars_bool b⟩], st ||)
+     | S_WhileTrue : forall st b s l sp,
+        (|| st, sp, WHILE b DO s END ||) --[l]-->s
+        (|| st, sp ++ [l⟨sym_beval st b, [], vars_bool b⟩], WHILE b DO s END ||)
         
     | S_WhileFalse : forall st b s l sp,
-        (|| WHILE b DO s END, sp, st ||) --[l]-->s
-        (|| SKIP, sp ++ [l⟨SymNot (sym_beval st b), [], vars_bool b⟩], st ||)                               
+        (|| st, sp, WHILE b DO s END ||) --[l]-->s
+        (|| st, sp ++ [l⟨SymNot (sym_beval st b), [], vars_bool b⟩],  SKIP ||)                               
 
     | S_N0While : forall st b n s l sp,
         n = 0 ->
-        (|| WHILE b FOR n DO s END, sp, st ||) --[l]-->s
-        (|| SKIP, sp, st ||)
+        (|| st, sp, WHILE b FOR n DO s END ||) --[l]-->s
+        (|| st, sp,  SKIP ||)
        
     | S_NWhileTrue : forall st b n s l sp,
-        (|| WHILE b FOR n DO s END, sp, st ||) --[l]-->s
-        (|| WHILE b FOR (n-1) DO s END, sp ++ [l⟨sym_beval st b, [], vars_bool b⟩], st ||)
+        (|| st, sp, WHILE b FOR n DO s END ||) --[l]-->s
+        (|| st, sp ++ [l⟨sym_beval st b, [], vars_bool b⟩], WHILE b FOR (n-1) DO s END ||)
                      
     | S_NWhileFalse : forall st b n s l sp,
-        (|| WHILE b FOR n DO s END, sp, st ||) --[l]-->s
-        (|| WHILE b FOR n DO s END, sp ++ [l⟨SymNot (sym_beval st b), [], vars_bool b⟩], st ||)
+        (|| st, sp, WHILE b FOR n DO s END ||) --[l]-->s
+        (|| st, sp ++ [l⟨SymNot (sym_beval st b), [], vars_bool b⟩], WHILE b FOR n DO s END ||)
 
-where " '(||' t ',' sp ',' st '||)' '--[' l ']-->s' '(||' t' ',' sp' ',' st' '||)'" :=
-        (sym_step (l) (t,sp,st) (t',sp',st')) . 
+where " '(||' st ',' sp ',' t '||)' '--[' l ']-->s' '(||' st' ',' sp' ',' t' '||)'" :=
+        (sym_step (l) (st,sp,t) (st',sp',t')) . 
 
 (*Example - one event*)
 Example sym_step_ex1 :
-  (|| X ::= 1, [] , (X !-> x(0)) ||) --[id 0]-->s
-  (|| SKIP, [id 0⟨SymBool true, [X], []⟩], (X !-> 1; X !-> x(0))||).
+  (|| (X |-> x(0)) , [] ,  X ::= 1 ||) --[id 0]-->s
+  (|| (X |-> 1; X |-> x(0)), [id 0⟨SymBool true, [X], []⟩], SKIP ||).
 Proof.
   apply S_Ass. Qed.
  
-Notation "'(||' t ',' sp ',' st '||)' '--[' l ']-->s*' '(||' t' ',' sp' ',' st' '||)'" :=
-   (multi (sym_step (l)) (t,sp, st) (t',sp',st'))
+Notation "'(||' st ',' sp ',' t '||)' '--[' l ']-->s*' '(||' st' ',' sp' ',' t' '||)'" :=
+   (multi (sym_step (l)) (st,sp, t) (st',sp',t'))
      (at level 40, st at level 39, t' at level 39).
 
 (*We do not care about the truth value of the events in the sympath, this is relevant when conncecting
@@ -167,11 +173,11 @@ concrete and symbolic evaluation*)
 
 (*Example - Choosing the false branch*)
 Example sym_step_if_false:
-  (|| stm_if, [] , (X !-> x(0); Y !-> y(0); Z !-> z(0)) ||) --[id 0]-->s*
-  (|| SKIP, [id 0⟨SymBool true, [X], []⟩ ;
+  (|| (X |-> x(0); Y |-> y(0); Z |-> z(0)), [] ,stm_if ||) --[id 0]-->s*
+  (|| (Z |-> 5; X |-> 1; X |-> x(0); Y |-> y(0); Z |-> z(0)),
+             [id 0⟨SymBool true, [X], []⟩ ;
              id 0⟨SymNot (1 < 1), [], [X]⟩;
-             id 0⟨SymBool true, [Z], []⟩],
-   (Z !-> 5; X !-> 1; X !-> x(0); Y !-> y(0); Z !-> z(0)) ||).
+             id 0⟨SymBool true, [Z], []⟩], SKIP ||).
 Proof.
   unfold stm_if.
   eapply multi_step. apply S_SeqStep. apply S_Ass. simpl.
@@ -182,12 +188,12 @@ Proof.
 (*Choosing the true branch*)
 Check (1 < 1). (*=> symExprBool*)
 Example sym_step_if_true:
-  (|| stm_if , [],  (X !-> x(0); Y !-> y(0); Z !-> z(0)) ||) --[id 0]-->s*
-  (|| SKIP, [id 0⟨SymBool true, [X], []⟩;
+  (|| (X |-> x(0); Y |-> y(0); Z |-> z(0)), [],  stm_if ||) --[id 0]-->s*
+  (|| (Y |-> 3; X |-> 1; X |-> x(0); Y |-> y(0); Z |-> z(0)),
+             [id 0⟨SymBool true, [X], []⟩;
              (*next we go on a different branch*)
              id 0⟨(1 < 1), [], [X]⟩;
-             id 0⟨SymBool true, [Y], []⟩],
-   (Y !-> 3; X !-> 1; X !-> x(0); Y !-> y(0); Z !-> z(0)) ||).
+             id 0⟨SymBool true, [Y], []⟩], SKIP ||).
 
 Proof.
   unfold stm_if.
@@ -198,54 +204,57 @@ Proof.
 
 (*symbolic evaluation of threads -> non-deterministc*)
 (*OBS: we always reduce to the first thread*)
-(*OBS:Where do we create the sym_paths?*)
-Reserved Notation "'(|' t ',' sp ',' st '|)' '-->ts' '(|' t' ',' sp' ',' st' '|)'"
+  (*OBS:Where do we create the sym_paths?*)
+
+(*Reserved Notation "'(||' st ',' sp ',' t '||)' '--[' l ']-->s' '(||' st' ',' sp' ',' t' '||)'"
+  (at level 40, st at level 39, t' at level 39). *)
+
+Reserved Notation "'(|' st ',' sp ',' t '|)' '-->ts' '(|' st' ',' sp' ',' t' '|)'"
          (at level 40, st at level 39, t' at level 39).
 
-Inductive tp_sym_step : (threadPool * symPath * sym_state) -> (threadPool * symPath * sym_state) -> Prop :=
-| S_T1 : forall st t1 t1' t2 st' sp sp',
-    (| t1, sp, st |) -->ts (| t1', sp', st' |) ->
-    (| (TPar t1 t2), sp, st |) -->ts
-    (| (TPar t1' t2), sp', st' |)
+Inductive tp_sym_step : (sym_state * symPath * threadPool ) -> (sym_state * symPath * threadPool ) -> Prop :=
+     | S_T1 : forall st t1 t1' t2 st' sp sp',
+        (| st, sp, t1 |) -->ts (| st', sp', t1' |) ->
+        (| st, sp, (TPar t1 t2) |) -->ts
+        (| st', sp', (TPar t1' t2) |)
     
-| S_T2 : forall st t1 t2 t2' st' sp sp',
-    (| t2, sp, st |) -->ts (| t2', sp', st' |) ->
-    (| (TPar t1 t2), sp, st |) -->ts
-    (| (TPar t1 t2'), sp', st' |)
+    | S_T2 : forall st t1 t2 t2' st' sp sp',
+        (| st, sp, t2 |) -->ts (| st', sp', t2' |) ->
+        (| st, sp, (TPar t1 t2) |) -->ts
+        (| st', sp', (TPar t1 t2') |)
    
     | S_ST1 : forall st s1 s1' st' n t2 sp sp', (*maybe i can use l instead of id n*)
         (*We need to initialise sym_paths*)
-        (|| s1, sp, st ||) --[id n]-->s (|| s1', sp', st' ||) ->
-        (| (TPar << id n | s1 >> t2), sp, st |)  -->ts
-        (| (TPar << id n | s1' >> t2), sp', st' |)
+        (|| st, sp, s1 ||) --[id n]-->s (|| st', sp', s1' ||) ->
+        (| st, sp, (TPar << id n | s1 >> t2) |)  -->ts
+        (| st', sp', (TPar << id n | s1' >> t2) |)
         
     | S_ST2 : forall st s2 s2' st' t1 n sp sp',
-        (|| s2, sp, st ||) --[id n]-->s (|| s2', sp', st' ||) ->
-        (| (TPar t1 << id n | s2 >>), sp, st |)  -->ts
-        (| (TPar t1 << id n | s2' >>), sp', st' |)
+        (|| st, sp, s2 ||) --[id n]-->s (|| st', sp', s2' ||) ->
+        (| st, sp, (TPar t1 << id n | s2 >>) |)  -->ts
+        (| st', sp', (TPar t1 << id n | s2' >>) |)
      
     | S_STDone : forall st n n' sp,
-        (| TPar << id n | SKIP >> << id n' | SKIP >>, sp, st |) -->ts
-        (| << id n | SKIP >>, sp, st |)                                                       
+        (| st, sp, (TPar << id n | SKIP >> << id n' | SKIP >>) |) -->ts
+        (| st, sp,  << id n | SKIP >> |)                                                       
         
-where "'(|' t ',' sp ',' st '|)' '-->ts' '(|' t' ',' sp' ',' st' '|)'" :=
-        (tp_sym_step (t, sp, st) (t', sp', st')). 
+where "'(|' st ',' sp ',' t '|)' '-->ts' '(|' st' ',' sp' ',' t' '|)'" :=
+        (tp_sym_step (st, sp, t) (st', sp', t')). 
 
-Notation " '(|' t ',' sp ',' st '|)' '-->ts*' '(|' t' ',' sp' ',' st' '|)'" :=
-   (multi tp_sym_step  (t,sp,st) (t',sp',st'))
+Notation " '(|' st ',' sp ',' t '|)' '-->ts*' '(|' st' ',' sp' ',' t' '|)'" :=
+   (multi tp_sym_step  (st,sp,t) (st',sp',t'))
      (at level 40, st at level 39, t' at level 39).
 
 (*We use the example on the article, generating sym_states and reducing sym_states 
 only on the true branches of the conditionals*)
 (*We do not have to take the computation untill the end but choose to do so here*)
 Example tpsym_article_true_brances :
-  (| example_article , [],  (X !-> x(0); Y !-> y(0)) |) -->ts*
-  (| << id 1 | SKIP >> ,
+  (| (X |-> x(0); Y |-> y(0)), [], example_article |) -->ts*
+  (| (X |-> 0 + 1 ; Y |-> 0 ; X |-> 0 ; X |-> x(0) ; Y |-> y(0)),
                [id 1⟨SymBool true, [X], []⟩;
                 id 2⟨(0 = 0), [], [X]⟩;
                 id 2⟨SymBool true, [Y], []⟩;
-                id 1⟨SymBool true, [X], [Y]⟩],
-               (X !-> 0 + 1 ; Y !-> 0 ; X !-> 0 ; X !-> x(0) ; Y !-> y(0)) |).
+                id 1⟨SymBool true, [X], [Y]⟩], << id 1 | SKIP >>|).
 Proof.
   unfold example_article.
   eapply multi_step. apply S_ST1. apply S_SeqStep. apply S_Ass. simpl.
@@ -258,7 +267,109 @@ Proof.
   eapply multi_step. eapply S_STDone.
   eapply multi_refl. Qed. 
 
-       
+(*we show "completeness" on a concrete example, the one in the article*)
+
+Check  (X !-> 1; Y !-> 0 ; X !-> 0). (*does not know we talk about concrete states*)
+Check (X |-> x(0) ; Y |-> y(0)).
+
+(*we could have a t' instead of << id 1 | SKIP >>. We might need inversion then*)
+(*Yes, we need inversion or induction on the t'*)
+
+(*Theorem exists_symbolic:
+    forall st st' t',
+    (*there are 2 valuations for which if i reach the end of the eval *)
+      (| st , example_article |) -->tc* (| st' , t' |) ->
+    exists st_s st_s' sp, 
+    (*I can find a symbolic evaluation for them*)  
+      (| st_s, [], example_article |) -->ts* (| st_s', sp, t' |).
+(*this is pretty independent from the concrete eval*)
+Proof.
+  (*inversion H usses multi and gives 2 cases, reflexivity and transitivity*)
+  unfold example_article. intros. induction t'. (*rewrite -> H3. *) *)
+  
+Theorem exists_symbolic_finish:
+    forall st st',
+    (*there are 2 valuations for which if i reach the end of the eval *)
+      (| st , example_article |) -->tc* (| st' , << id 1 | SKIP >> |) ->
+    exists st_s st_s' sp, 
+    (*I can find a symbolic evaluation for them*)  
+      (| st_s, [], example_article |) -->ts* (| st_s', sp, << id 1 | SKIP >>|).  
+  exists (X |-> x(0) ; Y |-> y(0)).
+  exists (X |-> 0 + 1 ; Y |-> 0 ; X |-> 0 ; X |-> x(0) ; Y |-> y(0)).
+  (*remember*) exists [id 1⟨SymBool true, [X], []⟩;
+                id 2⟨(0 = 0), [], [X]⟩;
+                id 2⟨SymBool true, [Y], []⟩;
+                id 1⟨SymBool true, [X], [Y]⟩].
+  eapply multi_step. apply S_ST1. apply S_SeqStep. apply S_Ass. simpl.
+  eapply multi_step. apply S_ST1. apply S_SeqFinish.
+
+  eapply multi_step. apply S_ST2. apply S_IfTrue. simpl. 
+  eapply multi_step. apply S_ST2. apply S_Ass.
+
+  eapply multi_step. apply S_ST1. apply S_Ass. simpl.
+  eapply multi_step. eapply S_STDone.
+  eapply multi_refl. Qed.
+
+(*Completenes??, do we want something specific as the end*)
+(*This will be hard to prove, I need someone that knows Coq*)
+Theorem completeness:
+    forall st st' t t',
+    (*there are 2 valuations for which if i reach the end of the eval *)
+      (| st , t |) -->tc* (| st' , t' |) ->
+    exists st_s st_s' sp, 
+    (*I can find a symbolic evaluation for them*)  
+      (| st_s, [], t |) -->ts* (| st_s', sp, t' |).
+Proof. Admitted.
+
+(*On the other way, from symbolic to concrete*)
+(*We need to collect the conditions*)
+
+Check id 1⟨SymBool true, [X], []⟩.
+Check (id 0⟨SymBool true, [], []⟩) :: []. 
+
+Fixpoint sym_cond (s: list event) : (list symExprBool) :=
+  match s with
+| [] => []
+| (i⟨e, wr, re⟩) :: t => [e] ++ sym_cond t
+  end.
+
+Compute (sym_cond  [id 0⟨SymBool true, [X], []⟩ ;
+             id 0⟨SymNot (x(0) < 1), [], [X]⟩;
+             id 0⟨SymBool true, [Z], []⟩]).
+
+(*the variables are in symaritt , we have to replace there *)
+Compute comp_LNat (x(0)) (x(0)).
+
+
+Reserved Notation "'[' x '::=' s ']' t" (at level 20).
+(*what should the result be*)
+(*cannot say for sure it is an aexpr, needs to be symExprArit*)
+(*we can make everything symExprArit and use constant folding*)
+(*another alternative is to assume that what we want to substitute is going to be there *)
+
+Fixpoint subst (x : SymLNat) (n : nat) (c : symExprArit) : aexpr := (*nat or SymAexpr*)
+  match c with
+  | SymLNat x' =>
+    if comp_LNat x x' then n else c
+  | SymNot b => negb (subst x n b)
+  | Sy
+                       
+  | var x' ⇒
+      if eqb_string x x' then s else t
+  | abs x' T t1 ⇒
+      abs x' T (if eqb_string x x' then t1 else ([x:=s] t1))
+  | app t1 t2 ⇒
+      app ([x:=s] t1) ([x:=s] t2)
+  | tru ⇒
+      tru
+  | fls ⇒
+      fls
+  | test t1 t2 t3 ⇒
+      test ([x:=s] t1) ([x:=s] t2) ([x:=s] t3)
+  end
+
+where "'[' x ':=' s ']' t" := (subst x s t).
+
 Close Scope symexpr. 
 Close Scope stm_scope.                           
 
